

Homework 1

Chen Peng

April 17, 2021

Exercise 1

Question 16.5.1: Find the second partial derivative of the following function

(2) $u = xy + \frac{y}{x}$

(4) $u = (xy)^z$

Answer:

(2) $\frac{\partial^2 u}{\partial x^2} = \frac{2y}{x^3}; \frac{\partial^2 u}{\partial x \partial y} = 1 - \frac{1}{x^2}; \frac{\partial^2 u}{\partial y^2} = 0$

(4) $\frac{\partial^2 u}{\partial x^2} = \frac{uz(z-1)}{x^2}; \frac{\partial^2 u}{\partial y^2} = \frac{uz(z-1)}{y^2}; \frac{\partial^2 u}{\partial z^2} = u(\ln x + \ln y)^2; \frac{\partial^2 u}{\partial x \partial y} = \frac{uz^2}{xy}; \frac{\partial^2 u}{\partial y \partial z} = \frac{uz}{y}(\ln x + \ln y) + \frac{u}{y};$
 $\frac{\partial^2 u}{\partial x \partial z} = \frac{uz}{x}(\ln x + \ln y) + \frac{u}{x}.$

Exercise 2

Question 16.5.2: Find the specified partial derivative of the following function:

(3) $u = x \ln(xy), \frac{\partial^3 u}{\partial x^2 \partial y};$

(7) $u = \ln \frac{1}{\sqrt{(x-\xi)^2 + (y-\eta)^2}}, \frac{\partial^4 u}{\partial x \partial y \partial \xi \partial \eta}$

Answer:

(3) 0

(7) $\frac{48(y-\eta)^2(x-\xi)^2}{((x-\xi)^2 + (y-\eta)^2)^4} - \frac{6}{((x-\xi)^2 + (y-\eta)^2)^2}$

Exercise 3

Question 16.5.7: Find the second partial derivative of the following function

(1) $u = f(ax, by);$

(2) $u = f(x + y, x - y);$

(3) $u = f(x + y, xy);$

(4) $u = f(x + y + z, x^2 + y^2 + z^2);$

(5) $u = f\left(\frac{x}{y}, \frac{y}{z}\right);$

(6) $u = f(x^2 + y^2 + z^2).$

Answer:

(1) $\frac{\partial^2 u}{\partial x^2} = a^2 f_{11};$

$\frac{\partial^2 u}{\partial x \partial y} = ab f_{12};$

$$\frac{\partial^2 u}{\partial y^2} = b^2 f_{22}$$

$$(2) \begin{aligned} \frac{\partial^2 u}{\partial x^2} &= f_{11} + 2f_{12} + f_{22}; \\ \frac{\partial^2 u}{\partial x \partial y} &= f_{11} - f_{22}; \\ \frac{\partial^2 u}{\partial y^2} &= f_{11} - 2f_{12} + f_{22} \end{aligned}$$

$$(3) \begin{aligned} \frac{\partial^2 u}{\partial x^2} &= f_{11} + 2yf_{12} + y^2 f_{22}; \\ \frac{\partial^2 u}{\partial x \partial y} &= f_{11} + f_2 + (x + y)f_{12} + xyf_{22}; \\ \frac{\partial^2 u}{\partial y^2} &= f_{11} + 2xf_{12} + x^2 f_{22} \end{aligned}$$

$$(4) \begin{aligned} \frac{\partial^2 u}{\partial x^2} &= f_{11} + 4xf_{12} + 2f_2 + 4x^2 f_{22}; \\ \frac{\partial^2 u}{\partial y^2} &= f_{11} + 4yf_{12} + 2f_2 + 4y^2 f_{22}; \\ \frac{\partial^2 u}{\partial z^2} &= f_{11} + 4zf_{12} + 2f_2 + 4z^2 f_{22}; \\ \frac{\partial^2 u}{\partial x \partial y} &= f_{11} + 2(x + y)f_{12} + 4xyf_{22}; \\ \frac{\partial^2 u}{\partial y \partial z} &= f_{11} + 2(y + z)f_{12} + 4yzf_{22}; \\ \frac{\partial^2 u}{\partial x \partial z} &= f_{11} + 2(x + z)f_{12} + 4xzf_{22}. \end{aligned}$$

$$(5) \begin{aligned} \frac{\partial^2 u}{\partial x^2} &= \frac{1}{y^2} f_{11}; \\ \frac{\partial^2 u}{\partial y^2} &= \frac{2x}{y^3} f_1 + \frac{x^2}{y^4} f_{11} - \frac{2x}{zy^2} f_{12} + \frac{1}{z^2} f_{22}; \\ \frac{\partial^2 u}{\partial z^2} &= \frac{2y}{z^3} f_2 + \frac{y^2}{z^4} f_{22}; \\ \frac{\partial^2 u}{\partial x \partial y} &= -\frac{1}{y^2} f_1 - \frac{x}{y^3} f_{11} + \frac{1}{zy} f_{12}; \\ \frac{\partial^2 u}{\partial y \partial z} &= -\frac{1}{z^2} f_2 + \frac{x}{yz^2} f_{12} - \frac{y}{z^3} f_{22}; \\ \frac{\partial^2 u}{\partial x \partial z} &= -\frac{1}{z^2} f_{12}. \end{aligned}$$

$$(6) \begin{aligned} \frac{\partial^2 u}{\partial x^2} &= 2f' + 4x^2 f''; \\ \frac{\partial^2 u}{\partial y^2} &= 2f' + 4y^2 f''; \\ \frac{\partial^2 u}{\partial z^2} &= 2f' + 4z^2 f''; \\ \frac{\partial^2 u}{\partial x \partial y} &= 4xyf''; \\ \frac{\partial^2 u}{\partial y \partial z} &= 4yzf''; \\ \frac{\partial^2 u}{\partial x \partial z} &= 4xzf''. \end{aligned}$$

Exercise 4

Question 16.5.16: Let $x = e^\xi$, $y = e^\eta$, transform equation:

$$ax^2 \frac{\partial^2 u}{\partial x^2} + 2bxy \frac{\partial^2 u}{\partial x \partial y} + cy^2 \frac{\partial^2 u}{\partial y^2} = 0$$

Answer:

$$\frac{\partial u}{\partial x} = \frac{1}{x} \frac{\partial u}{\partial \xi}, \quad \frac{\partial u}{\partial y} = \frac{1}{y} \frac{\partial u}{\partial \eta}$$

$$\frac{\partial^2 u}{\partial x^2} = \frac{1}{x^2} \left(\frac{\partial^2 u}{\partial \xi^2} - \frac{\partial u}{\partial \xi} \right), \quad \frac{\partial^2 u}{\partial y^2} = \frac{1}{y^2} \left(\frac{\partial^2 u}{\partial \eta^2} - \frac{\partial u}{\partial \eta} \right), \quad \frac{\partial^2 u}{\partial x \partial y} = \frac{1}{xy} \frac{\partial^2 u}{\partial \xi \partial \eta}$$

$$a \left(\frac{\partial^2 u}{\partial \xi^2} - \frac{\partial u}{\partial \xi} \right) + 2b \frac{\partial^2 u}{\partial \xi \partial \eta} + c \left(\frac{\partial^2 u}{\partial \eta^2} - \frac{\partial u}{\partial \eta} \right) = 0$$

Exercise 5

Question 16.5.20: Verify: No function satisfies

$$\frac{\partial f}{\partial x} = y, \quad \frac{\partial f}{\partial y} = x^2$$

Proof: Because

$$\frac{\partial}{\partial x} \left(\frac{\partial f}{\partial y} \right) = 2x \neq 1 = \frac{\partial}{\partial y} \left(\frac{\partial f}{\partial x} \right)$$

Exercise 6

Question 16.6.2: Find the Taylor expansion of $f(x, y) = x^2 + xy + y^2 + 3x - 2y + 4$ at $(-1, 1)$.

Answer:

$$\begin{aligned} f(x, y) &= (x + 1 - 1)^2 + (x + 1 - 1)(y - 1 + 1) + (y - 1 + 1)^2 + 3(x + 1 - 1) - 2(y - 1 + 1) + 4 \\ &= (x+1)^2 - 2(x+1) + 1 + (x+1)(y-1) - (y-1) + (x+1) - 1 + (y-1)^2 + 2(y-1) + 1 + 3(x+1) - 3 - 2(y-1) - 2 + 4 \\ &= 2(x+1) - (y-1) + (x+1)^2 + (x+1)(y-1) + (y-1)^2 \end{aligned}$$

Exercise 7

Question 16.6.3: Find the Taylor expansion of $f(x, y, z) = x^3 + y^3 + z^3 - 3xyz$ at $(1, 1, 1)$.

Answer:

$$\begin{aligned} f &= 3(x-1)^2 - 3(x-1)(z-1) - 3(y-1)(z-1) - 3(x-1)(y-1) \\ &\quad + (x-1)^3 + 3(y-1)^2 + (y-1)^3 + 3(z-1)^2 + (z-1)^3 - 3(x-1)(y-1)(z-1) \end{aligned}$$

Exercise 8

Question 16.6.6: Find the forth-order Taylor expansion of following functions at $(0, 0)$

(1) $u = \sin(x^2 + y^2)$;

(2) $u = \sqrt{1 + x^2 + y^2}$;

(3) $u = \ln(1 + x) \ln(1 + y)$;

(4) $u = e^x \cos y$.

Answer: (1)

$$u = x^2 + y^2 + o(\|h\|^4)$$

(2)

$$u = 1 + \frac{x^2}{2} + \frac{y^2}{2} - \frac{x^4}{8} - \frac{y^4}{8} - \frac{x^2 y^2}{4} + o(h^4)$$

(3)

$$u = xy - \frac{xy^2}{2} - \frac{x^2y}{2} + \frac{x^3y}{3} + \frac{xy^3}{3} + \frac{x^2y^2}{4} + o(h^4)$$

(4)

$$u = 1 + x + \frac{x^2}{2} - \frac{y^2}{2} + \frac{x^3}{6} - \frac{xy^2}{2} + \frac{x^4}{24} - \frac{x^2y^2}{4} + \frac{y^4}{24} + o(h^4)$$